\nonstopmode

%\RequirePackage{cleveref}

\newtheorem{theorem}{Theorem}
\newtheorem{proposition}[theorem]{Proposition}
\newtheorem{lemma}[theorem]{Lemma}
\newtheorem{corollary}[theorem]{Corollary}
\newtheorem{conjecture}[theorem]{Conjecture}
\newtheorem{definition}[theorem]{Definition}
\newtheorem{remark}[theorem]{Remark}
\newtheorem{example}[theorem]{Example}

\newcommand{\qed}{\ensuremath{\Box}}

\newenvironment{proof}[1][]{\noindent\ifthenelse{\equal{#1}{}}{\textit{Proof.}}{\textit{Proof #1.}}\hspace{2ex}}{\qed\bigskip}
\newenvironment{proof*}[1][]{\noindent\ifthenelse{\equal{#1}{}}{\textit{Proof.}}{\textit{Proof #1.}}\hspace{2ex}}{\bigskip}

% proof by cases
\newenvironment{caselist}{%
  \begin{list}{\textit{Case}}{}%
}{\end{list}%
}
\newenvironment{subcaselist}{%
  \begin{list}{\textit{Subcase}}{}%
}{\end{list}%
}
\newenvironment{subsubcaselist}{%
  \begin{list}{\textit{Subsubcase}}{}%
}{\end{list}%
}

\newcommand{\nextcase}{\item~}


%% Macros
\newcommand{\paradot}[1]{\paragraph*{#1.}}

\newcommand{\liftA}[1][]{\tliftA_{#1}}
\newcommand{\tliftA}{\mathsf{liftA}}
\newcommand{\compose}[2][]{\circ^{#1}_{#2}}
\newcommand{\tid}{\mathsf{id}}
\newcommand{\tfmap}{\mathsf{fmap}}
\newcommand{\fmap}[1]{\tfmap\,#1\,}
\newcommand{\tpure}{\mathsf{pure}}
\newcommand{\pure}{\tpure\,}
\newcommand{\law}[1]{\ensuremath{\mbox{\textbf{#1}}}}
\newcommand{\tApplicative}{\ensuremath{\mathsf{Applicative}}}
\newcommand{\idapp}{⊛}
\newcommand{\ulaw}[1]{\ensuremath{\mbox{\textit{#1}}}}


%% Content

%\newcommand{\MAIN}{Applicative}
\newcommand{\TITLE}{%
  An Agda Formalization of Applicative Functors
  Presented Via \texttt{liftA}$_n$}
\newcommand{\DATE}{17 January 2022}
\newcommand{\ABSTRACT}{
  McBride and Paterson \citeyearpar{mcBridePaterson:jfp08}
  introduced \texttt{Applicative} functors to
  Haskell, which are equivalent to the lax monoidal functors (with
  strength) of category theory.  Applicative functors $F$ are presented
  via \emph{idiomatic application} $\_⊛\_ : F(A → B) → FA → FB$ and
  laws that look ad-hoc and hard to remember.  We propose instead to
  define applicative functors by a family $\liftA[n] : (A_1 \to \dots
  \to A_n \to C) \to FA_1 \to \dots \to FA_n \to FC$ of
  \texttt{zipWith}-like functions that generalize \texttt{pure} $(n=0)$,
  \texttt{fmap} $(n=1)$ and \texttt{liftA2} $(n=2)$.  This reduces the
  associated laws to just the first functor law and one composition
  law for $\liftA$.
}
\newcommand{\INTRO}{%

\section{Introduction}

\citet{mcBridePaterson:jfp08} introduce applicative functors as a
Haskell type constructor class $\Applicative~F$ with two methods
\[
\begin{array}{llll}
  \tpure & : & A \to F\,A
    & \mbox{embedding} \\
  \_\idapp\_ & : & F\,(A \to B) \to F\,A \to F\,B
    & \mbox{idiomatic application, left associative} \\
\end{array}
\]
satisfying four laws:
\[
\begin{array}{l@{\qquad}lll}
  \ulaw{identity}
    & \pure \tid \idapp u & = & u
\\
  \ulaw{composition}
    & \pure (\_{\circ}\_) \idapp u \idapp v \idapp w
    & = & u \idapp (v \idapp w)
\\
  \ulaw{homomorphism}
    & \pure f \idapp \pure x & = & \pure (f\,x)
\\
  \ulaw{interchange}
    & u \idapp \pure x
    & = & \pure (\lambda f \to f x) \idapp u
\end{array}
\]
Herein, $\tid = \lambda x \to x$ is the identity function and $(f \circ
g)\,x = f\,(g\,x)$ unary function composition.

Functoriality of $F$ is recovered via $\fmap f u = \pure f \idapp u$
where \ulaw{identity} acts as the first functor law.  The second
functor law can be derived via \ulaw{composition} and
\ulaw{homomorphism} as follows:
\[
\begin{array}{llllll}
  \fmap f (\fmap g u)
    & = & \pure f \idapp (\pure g \idapp u)
    & = & \pure (\_\circ\_) \idapp \pure f \idapp \pure g \idapp u \\
    & = & \pure (f \circ\_) \idapp \pure g \idapp u
    & = & \pure (f \circ g) \idapp u \\
    & = & \fmap {(f \circ g)} u
\end{array}
\]

Unfortunately, \citeauthor{mcBridePaterson:jfp08}'s laws are not easy
to remember, especially the \ulaw{composition} and \ulaw{interchange}
laws.  The do not follow simple patterns like the functor laws which
can be seen as actions of the function category, or the monad laws,
which can be conceived as generalization of the monoid laws.  It is
also not intuitively clear at a glance that these laws are complete.

Starting with GHC 8.2, $\tApplicative$s can also be given via
$\liftA[2] : (A \to B \to C) \to FA \to FB \to FC$
rather than idiomatic application, which are
interdefinable:
\[
\begin{array}{lll}
  \liftA[2]\,f\,u\,v & = & \pure f \idapp u \idapp v \\
  h \idapp u         & = & \liftA[2]\,(\lambda f x \to f x)\,h\,u \\
\end{array}
\]
However, to this date (2022-01-18) the documentation of
$\tApplicative$ does not spell out the type class laws in terms of
$\liftA[2]$.

Note that $\liftA[2]$ appears to be the \emph{binary} generalization
of the \emph{unary} $\tfmap = \liftA[1] : (A \to B) \to FA \to FB$.
In the same way, we get the \emph{nullary} $\tpure = \liftA[0] : A \to
FA$.

In this note, we show that the further generalization to arbitrary
arities $\liftA[n]$ gives very elegant laws for the familty
$\liftA[n]$, which are just generalizations of the two functor laws.

\section{Applicative Functors as Arity-Generalized Functors}

\paradot{Preliminaries: generalized composition}
If $f : A_{1..n} \to C \to D$ and $g : B_{1..m} \to C$ then let
$f \compose[m]n g : A_{1..n} \to B_{1..m} \to D$ be
defined by
\[
  (f \compose[m]n g)\;a_{1..n}\;b_{1..m} = f\,a_{1..n}\,(g\,b_{1..m})
  .
\]
Herein, $h\,x_{1..n}$ is to be understood as curried application
$h\,x_1\,\dots\,x_n$.  A sequence $x_{1..n}$ may more succinctly be
written as $\vec x^n$ or just $\vec x$.

Note that $(f \compose[1]0 g)\,x = f\,(g\,x)$ is ordinary unary function composition.
Further, $(f \compose[0]n y)\,a_{1..n} = f\,a_{1..n}\,y$ is partial application of $f$ to its $n+1$st argument, which for $n=0$ is just plain application: $f \compose[0]0 y = f\,y$.
% If $f : A_{1..n} \to B \to C_{1..\ell} \to D$ and $g : B_{1..m} \to B$ then
% $f \compose[n]{m}k g : A_{1..n} \to B_{1..m} \to C_{1..\ell} \to D$.
% We define $(f \compose m k g)\;a_{1..n}\;b_{1..m} = f\,a_{1..n}\,(g\,b_{1..m})$.

\paradot{Arity-generalized functors}
To distinguish our concept of applicative functors from that of
\citeauthor{mcBridePaterson:jfp08}, we temporarily call them
\emph{arity-generalized functor}.

An arity-generalized functor $F$ shall be witnessed by a family of functions
\[
  \liftA[n] :
    (A_1 \to \dots \to A_n \to C) \to FA_1 \to \dots \to FA_n \to FC
\]
satisfying the following laws:
\[
  \begin{array}{l@{\qquad}l@{~~}l@{~~}l}
\law{identity} & \liftA[1]\,\tid & = & \tid \\
\law{composition}
  & \liftA[n+1+m]\,f\,\vec u^n\,(\liftA[k]\,g\,\vec v^k)
  & =
  & \liftA[n+k+m]\,(f \compose[k]n g)\,\vec u\, \vec v
  % & \liftA[n+1+m]\,f\,u_{1..n}\,(\liftA[k]\,g\,v_{1..k}) %\,w_{1..m}
  % & =
  % & \liftA[n+k+m]\,(f \compose[k]n g)\,u_{1..n}\,v_{1..k} %\,w_{1..m}
  \end{array}
\]
%
We may % take the liberty of writing a sequence $u_{1..n}$ as just
% $\vec u^n$ or $\vec u$ and
drop the index to $\tliftA$ when it is
generic or clear from the context of discourse.

Just functoriality of $F$ can be recovered by $\tfmap = \liftA[1]$ with \law{identity} being the first functor law and \law{composition} specializing to the second functor law with $n=m=0$ and $k=1$:
\[
  \liftA[1]\,f\,(\liftA[1]\,g\,v) = \liftA[1]\,(f \compose[1]0 g)\,v
\]
Pure computations are represented via $\tpure = \liftA[0]$, with the composition law specializing to:
\[
%  \liftA[n+1+m]\,f\,u_{1..n}\,(\tpure\, x)\,w_{1..m}
  \liftA\,f\,\vec u^n\,(\pure x) %\,\vec w
  =
  \liftA\,(f \compose[0]n x)\,\vec u %\,\vec w
\]
For $\tfmap$ ($n = m = 0$) this yields $\fmap f (\pure x) = \pure (f\,x)$.
%
For just $n=0$ we get law $\liftA[1+m]\,f\,(\pure x)\,\vec w =
\liftA[m]\,(f\,x)\,\vec w$. This can be iterated to
$\liftA[n]\,f\,(\tpure\,x_1)\,\dots\,(\tpure\,x_n) =
\tpure\,(f\,x_{1..n})$ corresponding to the intuition that composition
of effect-free computations is again an effect-free computation.

\subsection{Arity-generalized functors are applicative}

Idiomatic application can be obtained as a special case of
$\liftA[2]$:
\[
\begin{array}{lll}
  \_\idapp\_ & : & F (A \to B) \to F A \to F B \\
  u \idapp v & = & \liftA[2]\,\tid\,u\,v
\end{array}
\]
We easily derive its laws:
\begin{enumerate}

\item \ulaw{identity}:
\[
\begin{array}{lllllll@{\qquad}l}
  \pure \tid \idapp u
    & = & \liftA[2]\,\tid\,(\pure \tid)\, u
    & = & \liftA[1]\,(\tid \compose[0]{0} \tid)\, u
    &&
    & \mbox{by \law{composition}}
\\
    & = & \liftA[1]\,(\tid \, \tid)\, u
    & = & \liftA[1]\,\tid\, u
    & = & u
    & \mbox{by \law{identity}}
\\
\end{array}
\]

\item \ulaw{composition}.
\[
\begin{array}{lllll@{\qquad}l}
\multicolumn{6}{l}{
  \pure (\_{\circ}\_) \idapp u \idapp v \idapp w
}
\\
    & = & \liftA[2]\,\tid\,(\pure (\_{\circ}\_)\, u \idapp v \idapp w
    & = & \liftA[1]\,(\_{\circ}\_)\,u \idapp v \idapp w
    & \mbox{by \law{composition}}
\\
    & = & \liftA[2]\,\tid\,(\liftA[1]\,(\_{\circ}\_)\,u)\,v \idapp w
    & = & \liftA[2]\,(\_{\circ}\_)\,u\,v \idapp w
    & \mbox{by \law{composition}}
\\
    & = & \liftA[2]\,\tid\,(\liftA[2]\,(\_{\circ}\_)\,u\,v)\,w
    & = & \liftA[3]\,(\_{\circ}\_)\,u\,v\,w
    & \mbox{by \law{composition}}
\\
    & = & \liftA[3]\,(\lambda f g x \to f\,(g x))\,u\,v\,w
    & = & \liftA[3]\,(\lambda f g x \to \tid\,f\,(\tid\,g\,x))\,u\,v\,w
\\
    & = & \liftA[3]\,(\tid \compose[2]1 \tid)\,u\,v\,w
    & = & \liftA[2]\,\tid\,u\,(\liftA[2]\,\tid\,v\,w)
    & \mbox{by \law{composition}}
\\
    & = & u \idapp (v \idapp w)
\end{array}
\]


\item \ulaw{homomorphism}.  This has been shown before, here again step-by-step:
\[
\begin{array}{lllll@{\qquad}l}
  \pure f \idapp \pure x
    & = & \liftA[2]\,\tid\,(\pure f)\,(\pure x)
    & = & \liftA[1]\,(\tid\,f)\,(\pure x)
    & \mbox{by \law{composition}}
\\
    & = & \liftA[1]\,f\,(\pure x)
    & = & \liftA[0]\,(f\,x)
    & \mbox{by \law{composition}}
\\
    & = & \pure\,(f\,x)
\end{array}
\]

\item \ulaw{interchange}:
\[
\begin{array}{lllll@{\qquad}l}
  u \idapp (\pure x)
    & = & \liftA[2]\,\tid\,u\,(\liftA[0]\,x)
    & = & \liftA[1]\,(\tid \compose[0]{1} x)\,u
    & \mbox{by \law{composition}}
\\
    & = & \liftA[1]\,(\lambda f \to f\,x)\,u
    & = & \pure (\lambda f \to f x) \idapp u
    & \mbox{by \law{composition}}
\end{array}
\]


\end{enumerate}

%% With $h

\subsection{Applicative functors are arity-generalized}

Following \citet{mcBridePaterson:jfp08}, the family $\liftA[n]$ can be
defined for each applicative functor:
\[
\begin{array}{lll}
  \liftA[0]  \,x & = & \pure x \\
  \liftA[n+1]\,f\,\vec u\,v & = & \liftA[n]\,f\,\vec u \idapp v
\end{array}
\]
The \law{identity} is just \ulaw{identity}. We establish
\law{composition} by a series of inductions.

\begin{lemma}[Frame]
  \label{lem:frame}
  If\/ $\liftA[n]\,f\,\vec u^n = \liftA[k]\,g\,\vec v^k$ then
  $\liftA[n+m]\,f\,\vec u\,\vec w^m = \liftA[k+m]\,g\,\vec v\,\vec w$.
\end{lemma}
\begin{proof}
  By induction on $m$.
\end{proof}

As a consequence of \Cref{lem:frame}, we only need to show the composition law for $m=0$:
\[
  \liftA[n+1]\,f\,\vec u^n\,(\liftA[k]\,g\,\vec v^k)
  =
  \liftA[n+k]\,(f \compose[k]n g)\,\vec u\, \vec v
\]
We first show the case $n=0$:
\begin{lemma}[Composition for $n=0$]
\[
  \liftA[1]\,f\,(\liftA[k]\,g\,\vec v) = \liftA[k]\,(f \compose[k]0 g)\,\vec v
\]
\end{lemma}
\begin{proof*}
By induction on $k$.
\begin{caselist}
\nextcase $k=0$: This is \ulaw{homomorphism}.
\nextcase $k \to k+1$.
\[
\begin{array}{lllll@{\qquad}l}
\multicolumn 6 l {
  \liftA[1]\,f\,(\liftA[k+1]\,g\,\vec v\,w)
}\\
    & = & \pure f \idapp (\liftA[k]\,g\,\vec v \idapp w)
\\
    & = & \pure (\_{\circ}\_) \idapp \pure f \idapp \liftA[k]\,g\,\vec v \idapp w
    & \mbox{by \ulaw{composition}}
\\
    & = & \pure (f \circ \_) \idapp \liftA[k]\,g\,\vec v \idapp w
    &&
    & \mbox{by \ulaw{homomorphism}}
\\
    & = & \liftA[k]\,((f \circ \_) \compose[k]0 g)\,\vec v \idapp w
    &&
    & \mbox{by ind.hyp.}
\\
    & = & \liftA[k+1]\,(f \compose[k+1]0 g)\,\vec v\, w
\end{array}
\]
For the last step, note that
\(
  (f \circ \_) \compose[k]0 g
  = \lambda \vec x^k \to (f \circ \_) (g\,\vec x)
  = \lambda \vec x \to f \circ (g\,\vec x)
  = \lambda \vec x y \to f (g\,\vec x\,y)
  = f \compose[k+1]0 g
\).
\qed
\end{caselist}
\end{proof*}

\begin{corollary}[Composition for $k=0$]
\[
  \liftA[n+1]\,f\,\vec u\,(\pure x)
  = \liftA[n]\,(f \compose[0]n x)\,\vec u
\]
\end{corollary}
\begin{proof*}
\[
\begin{array}{lllll@{\qquad}l}
\multicolumn 6 l {
  \liftA[n+1]\,f\,\vec u\,(\pure x)
}\\
    & = & \liftA[n]\,f\,\vec u \idapp \pure x
    & = & \pure (\lambda k \to k\,x) \idapp \liftA[n]\,f\,\vec u
    & \mbox{by \ulaw{exchange}}
\\
    & = & \liftA[n]\,((\lambda k \to k\,x) \compose[n]0 f)\,\vec u
    & = & \liftA[n]\,(f \compose[0]n x)\,\vec u
\end{array}
\]
The last step is justified by
\(
    (\lambda k \to k\,x) \compose[n]0 f
  = \lambda \vec y^k \to (\lambda k \to k\,x)\,(f \vec y)
  = \lambda \vec y^k \to f \vec y\,x
  = f \compose[0]n x
\).
\qed
\end{proof*}

\begin{lemma}[Composition for $n=k=0$]
\label{lem:comp}
\(
  \liftA[1+m]\,f\,(\pure x)\,\vec w = \liftA[m]\,(f\,x)\,\vec w
  .
\)
\end{lemma}
\begin{proof*}
By induction on $m$:
\begin{caselist}
\nextcase $m=0$:  This is the \ulaw{homomorphism} law.
\[
\begin{array}{lllllll}
  \liftA[1]\,f\,(\pure x)
    & = & \pure f \idapp \pure x
    & = & \pure\,(f x)
    & = & \liftA[0]\,(f\,x)
\end{array}
\]
\nextcase $m \to m+1$:
\[
\begin{array}{lll@{\qquad}l}
%\multicolumn 5 l {
  \liftA[1+m+1]\,f\,(\pure x)\,\vec w\,w
%}
%\\
    & = & \liftA[1+m]\,f\,(\pure x)\,\vec w \idapp w
\\
    & = & \liftA[m]\,(f\,x)\,\vec w \idapp w
    & \mbox{by ind.hyp.}
\\
    & = & \liftA[m+1]\,(f\,x)\,\vec w\, w
\end{array}
\]
\qed
\end{caselist}
\end{proof*}

\begin{lemma}[Composition for $k=0$]
\[
  \liftA[n+1]\,f\vec u\,(\pure x)
  = \liftA[n]\,(f \compose[0]n x)\,\vec u
\]
\end{lemma}
\begin{proof*}
By induction on $n$:
\begin{caselist}
\nextcase $n=0$: This is \ulaw{homomorphism}.
\nextcase $n \to n+1$.
\qed
\end{caselist}
\end{proof*}


\section{The development}
}
\newcommand{\CONCLUSION}{%
  Q.E.D.
  \par
  \paragraph*{Acknowledgments.}
  \GENERATED
\bibliographystyle{abbrvnat}
\bibliography{auto-Applicative}
}

\input{template}

%%% Local Variables:
%%% coding: utf-8
%%% mode: latex
%%% TeX-engine: xetex
%%% TeX-master: t
%%% End:
